\appendix
\section{Logic}\label{appendix:Logic}
De Morgan rules:
\begin{align*}
    \alpha \land \beta &\equiv \beta \land \alpha \\
    \alpha \lor \beta &\equiv \beta \lor \alpha \\
    (\alpha \land \beta)\land \gamma &\equiv \alpha \land (\beta \land \gamma) \\
    (\alpha \lor \beta)\lor \gamma &\equiv \alpha \lor (\beta \lor \gamma) \\
    \neg (\neg \alpha) &\equiv \alpha \\
    \alpha \Rightarrow \beta &\equiv \neg \beta \Rightarrow \neg \alpha \\
    \alpha \Rightarrow \beta &\equiv \neg \alpha \lor \beta \\
    \alpha\Leftrightarrow\beta &\equiv (\alpha\Rightarrow\beta) \land (\beta\Rightarrow\alpha) \\
    \neg (\alpha \land \beta) &\equiv (\neg \alpha \lor \neg \beta) \\
    \neg (\alpha \lor \beta) &\equiv (\neg \alpha \land \neg \beta) \\
    \alpha \land (\beta \lor \gamma) &\equiv (\alpha\land\beta)\lor(\alpha\land\gamma) \\
    \alpha \lor (\beta \land \gamma) &\equiv (\alpha \lor \beta)\land(\alpha \lor \gamma)
\end{align*}